src/Linear.v
@@ -1,0 +1,167 @@
+Require Import Bool List String Peano_dec.
+Require Import Permutation.
+Require Import Common FMap Syntax Semantics.
+
+(* In message passing system, a "process" (or "thread") refers to a 
+ * "requester" and an "objects" (or "system") refers to a "requestee".
+ * Thus, for a given message {| mid_rq := i; mid_rs := j; mid_rqrs := _ |},
+ * its requester (process) is "i" and the (target) object is "j".
+ *)
+
+(* [sys] acts as a processor for [msg]. *)
+Definition asProcessor (sys: System) (msg: Msg) :=
+  if mid_rq (msg_id msg) ?<n (indicesOf sys) then true else false.
+Definition asSystem (sys: System) (msg: Msg) :=
+  if mid_rs (msg_id msg) ?<n (indicesOf sys) then true else false.
+
+Definition sysSubHistory (sys: System) (hst: list Msg) :=
+  filter (asSystem sys) hst.
+Definition procSubHistory (sys: System) (hst: list Msg) :=
+  filter (asProcessor sys) hst.
+
+(* For a given system [sys] and its trace [tr], the history of [tr] is an
+ * object subhistory with respect to [sys], where [lbl_hdl] is ignored.
+ *)
+Fixpoint historyOf (sys: System) (tr: Trace) :=
+  match tr with
+  | nil => nil
+  | {| elbl_ins := ins; elbl_outs := outs |} :: tr' =>
+    (sysSubHistory sys (outs ++ ins)) ++ (historyOf sys tr')
+  end.
+
+Inductive History : System -> list Msg -> Prop :=
+| Hist: forall sys hst,
+    Behavior sys hst ->
+    History sys (historyOf sys hst).
+
+(* A history consisting only of requests and matching responses. *)
+Inductive Complete: list Msg -> Prop :=
+| CplNil: Complete nil
+| CplAdd:
+    forall hst1 hst2 hst3,
+      Complete (hst1 ++ hst2 ++ hst3) ->
+      forall rq rs,
+        isTrsPair (msg_id rq) (msg_id rs) = true ->
+        forall chst,
+          chst = hst1 ++ rq :: hst2 ++ rs :: hst3 ->
+          Complete chst.
+
+Inductive SubHistory {A}: list A -> list A -> Prop :=
+| SlNil: SubHistory nil nil
+| SlAdd: forall l1 l2, SubHistory l1 l2 -> forall a, SubHistory (a :: l1) (a :: l2)
+| SlSkip: forall l1 l2, SubHistory l1 l2 -> forall a, SubHistory l1 (a :: l2).
+
+Definition ExtHistory {A} (l el: list A): Prop :=
+  exists e, el = l ++ e.
+
+Fixpoint matchTrsPair (rq: Msg) (rss: list Msg) :=
+  match rss with
+  | nil => None
+  | rs :: rss' =>
+    if isTrsPair (msg_id rq) (msg_id rs) then Some rss'
+    else match matchTrsPair rq rss' with
+         | Some nrss => Some (rs :: nrss)
+         | None => None
+         end
+  end.
+
+(* Assuming the history is well-formed. *)
+Fixpoint complete' (hst rss: list Msg): list Msg * list Msg :=
+  match hst with
+  | nil => (nil, rss)
+  | msg :: hst' =>
+    match mid_rqrs (msg_id msg) with
+    | Rq => let (phst, prss) := complete' hst' rss in
+            match matchTrsPair msg prss with
+            | Some nrss => (msg :: phst, nrss)
+            | None => (phst, prss)
+            end
+    | Rs => let (phst, prss) := complete' hst' rss in
+            (msg :: phst, msg :: prss)
+    end
+  end.
+
+Definition complete (hst: list Msg) := fst (complete' hst nil).
+Definition WellFormed (hst: list Msg) := snd (complete' hst nil) = nil.
+
+Lemma complete_subList: forall hst, SubHistory (complete hst) hst.
+Proof.
+Admitted.
+
+Lemma complete_complete: forall hst, Complete (complete hst).
+Proof.
+Admitted.
+
+Lemma complete_maximal:
+  forall hst chst,
+    chst <> complete hst ->
+    SubHistory chst hst -> Complete chst ->
+    ~ SubHistory (complete hst) chst.
+Proof.
+Admitted.
+
+(* An informal definition of "sequential":
+ * 1) The first message should be a request
+ * 2) A matching response for each request should be right after the request.
+ * 3) There might not be a matching response for the last request.
+ *)
+Fixpoint Sequential' (hst: list Msg) (orq: option Msg) :=
+  match hst with
+  | nil => true
+  | msg :: hst' =>
+    match orq with
+    | Some rq => isTrsPair (msg_id rq) (msg_id msg) && Sequential' hst' None
+    | None => match mid_rqrs (msg_id msg) with
+              | Rq => Sequential' hst' (Some msg)
+              | Rs => false
+              end
+    end
+  end.
+Definition Sequential (hst: list Msg) := Sequential' hst None = true.
+Definition Concurrent (hst: list Msg) := ~ Sequential hst.
+
+Definition sequential_concurrent_dec:
+  forall hst, {Sequential hst} + {Concurrent hst}.
+Proof.
+  unfold Concurrent, Sequential; intros.
+  destruct (Sequential' hst None).
+  - left; reflexivity.
+  - right; discriminate.
+Defined.
+
+(* A system is sequential when all possible histories are sequential. *)
+Definition SequentialSys (sys: System) :=
+  forall hst, History sys hst -> Sequential (rev hst).
+
+Definition requestsOf (hst: list Msg) :=
+  filter (fun m => match mid_rqrs (msg_id m) with
+                   | Rq => true
+                   | _ => false
+                   end) hst.
+
+(* Two histories are equivalent if
+ * 1) one history is a permutation of the other, and
+ * 2) they have the same request orders per a process.
+ *)
+Definition Equivalent (hst1 hst2: list Msg) :=
+  Permutation hst1 hst2 /\
+  forall obj, requestsOf (procSubHistory [obj] hst1) =
+              requestsOf (procSubHistory [obj] hst2).
+
+(* NOTE: this is actually not a fully correct definition:
+ * Linearizability requires one more condition: any _strict_ transaction
+ * orders are preserved by [lhst].
+ * I'm currently not sure if we need the second condition for 
+ * message-passing systems.
+ *)
+Definition Linearizable (hst lhst: list Msg) :=
+  Sequential lhst /\
+  Equivalent (complete hst) lhst.
+
+(* A system is linear when all possible histories are linearizable. *)
+Definition Linear (sys: System) :=
+  forall hst,
+    History sys hst ->
+    exists lhst, History sys lhst /\
+                 Linearizable (rev hst) (rev lhst).
+
