src/Synthesis.v
@@ -1,24 +1,19 @@
 Require Import Bool List String Peano_dec.
-Require Import Common FMap Syntax Semantics.
-
-Definition OInvariant := M.t (StateT -> Prop).
-
-Definition OInvariantHolds (inv: OInvariant) (oss: ObjectStates) :=
-  forall idx,
-    match inv@[idx], oss@[idx] with
-    | Some oinv, Some os => oinv os
-    | _, _ => True
-    end.
-
-Record OInvariants (sys: System) :=
-  { oinv_inv : OInvariant;
-    oinv_init : OInvariantHolds oinv_inv (getObjectStatesInit (sys_objs sys)) }.
+Require Import Common FMap Syntax Semantics Simulation.
 
 Section Synthesis.
 
   (** Requirements *)
-  Variables (sys: System) (* a topology among objects *)
-            (invs: OInvariants sys).
+  Variables
+    (impl0 spec: System) (* an initial system and the spec *)
+    (R: State -> State -> Prop)
+    (Hrinit: R (getStateInit impl0) (getStateInit spec))
+    (Hsim: Simulates R impl0 spec). (* a simulation relation *)
+
+  Lemma impl0_ok: impl0 ⊑ spec.
+  Proof.
+    eapply simulation_implies_refinement; eauto.
+  Qed.
 
 End Synthesis.
 
